More proof

inductive_proof/Queue_set/App.fst
@@ -1,19 +1,19 @@
 module App
 
 open SeqUtils
-open Set_extended
+module S = Set_extended
 
 #set-options "--query_stats"
 // the concrete state type
 // It is a set of pairs of timestamp and element.
-type concrete_st = s:set (nat & nat)//{s <> empty ==> (exists (e:(nat * nat)). mem e s /\ (forall e1. mem e1 s ==> fst e <= fst e1))}
+type concrete_st = s:S.set (nat & nat)//{s <> empty ==> (exists (e:(nat * nat)). mem e s /\ (forall e1. mem e1 s ==> fst e <= fst e1))}
 
 // init state
-let init_st = empty
+let init_st = S.empty
 
 // equivalence between 2 concrete states
 let eq (a b:concrete_st) =
-  (forall e. mem e a <==> mem e b)
+  S.equal a b
 
 // few properties of equivalence relation
 let symmetric (a b:concrete_st) 
@@ -41,39 +41,39 @@ let get_ele (o:op_t{Enqueue? (fst (snd o))}) : nat =
   |(_, (Enqueue x,_)) -> x
 
 let mem_id_s (id:nat) (s:concrete_st) =
-  exists_s s (fun e -> fst e = id)
-
+  S.exists_s s (fun e -> fst e = id)
+  
 let unique_st (s:concrete_st) =
   //forall_s s (fun e -> count e s > 0) &&
-  forall_s s (fun e -> not (exists_s s (fun e1 -> snd e <> snd e1 && fst e = fst e1)))
+  S.forall_s s (fun e -> not (S.exists_s s (fun e1 -> snd e <> snd e1 && fst e = fst e1)))
 
-val extract_s (m:option (nat * nat){Some? m}) : nat * nat
+val extract_s (#a:Type0) (m:option a{Some? m}) : a
 let extract_s (Some x) = x
 
 let find_min (s:concrete_st)
     : (m:option (nat * nat) 
-           {(Some? m <==> (exists (e:(nat * nat)). mem e s /\ (forall e1. mem e1 s ==> fst e <= fst e1))) /\
-            (Some? m ==> (exists (e:(nat * nat)). mem e s /\ (forall e1. mem e1 s ==> fst e <= fst e1) /\ e = extract_s m)) /\
-        (s = empty ==> (m = None \/ (~ (exists (e:(nat * nat)). mem e s /\ (forall e1. mem e1 s ==> fst e <= fst e1))))) 
+           {(Some? m <==> (exists (e:(nat * nat)). S.mem e s /\ (forall e1. S.mem e1 s ==> fst e <= fst e1))) /\
+            (Some? m ==> (exists (e:(nat * nat)). S.mem e s /\ (forall e1. S.mem e1 s ==> fst e <= fst e1) /\ e = extract_s m)) /\
+        (s = S.empty ==> (m = None \/ (~ (exists (e:(nat * nat)). S.mem e s /\ (forall e1. S.mem e1 s ==> fst e <= fst e1))))) 
         (*s <> empty ==> Some? m*)}) =
-  find_if s (fun e -> (forall_s s (fun e1 -> fst e <= fst e1)))
+  S.find_if s (fun e -> (S.forall_s s (fun e1 -> fst e <= fst e1)))
 
 let check_find_min (s:concrete_st)
-  : Lemma (requires s = add (2,1) (singleton (3,1)))
+  : Lemma (requires s = S.add (2,1) (S.singleton (3,1)))
           (ensures find_min s = Some (2,1)) 
   = let m = find_min s in
-    assert (mem (2,1) s /\ (forall e1. mem e1 s ==> fst (2,1) <= fst e1));
+    assert (S.mem (2,1) s /\ (forall e1. S.mem e1 s ==> fst (2,1) <= fst e1));
     (*assert (Some? m);
     assert (fst (extract_s m) = 1);
     assert (forall e. mem e s ==> 1 <= fst e);*) ()
 
 let remove_min (s:concrete_st) 
-  : (r:concrete_st{(s = empty ==> r = s) /\
-                   (s <> empty /\ Some? (find_min s) ==> (forall e. mem e r <==> (mem e s /\ e <> extract_s (find_min s)))) /\
-                   (s <> empty /\ None? (find_min s) ==> (forall e. mem e r <==> mem e s))}) =
-  if s = empty then s 
+  : (r:concrete_st{(s = S.empty ==> r = s) /\
+                   (s <> S.empty /\ Some? (find_min s) ==> (forall e. S.mem e r <==> (S.mem e s /\ e <> extract_s (find_min s)))) /\
+                   (s <> S.empty /\ None? (find_min s) ==> (forall e. S.mem e r <==> S.mem e s))}) =
+  if s = S.empty then s 
   else (let m = find_min s in
-        if Some? m then remove_if s (fun e -> e = extract_s (find_min s))
+        if Some? m then S.remove_if s (fun e -> e = extract_s (find_min s))
         else s)
 
 let find_min_equal (a b:concrete_st)
@@ -83,8 +83,8 @@ let find_min_equal (a b:concrete_st)
 // apply an operation to a state
 let do (s:concrete_st) (op:op_t) : concrete_st =
   match op with
-  |(id, (Enqueue x, _)) -> add (id, x) s
-  |(_, (Dequeue, _)) -> if s = empty then s else remove_min s
+  |(id, (Enqueue x, _)) -> S.add (id, x) s
+  |(_, (Dequeue, _)) -> if s = S.empty then s else remove_min s
 
 let lem_do (a b:concrete_st) (op:op_t)
    : Lemma (requires eq a b)
@@ -97,8 +97,8 @@ let lem_do (a b:concrete_st) (op:op_t)
 let return (s:concrete_st) (o:op_t) : ret_t =
   match o with
   |(_, (Enqueue _, _)) -> None
-  |(_, (Dequeue, r)) -> if s = empty then None 
-                          else (assume (exists (e:(nat * nat)). mem e s /\ (forall e1. mem e1 s ==> fst e <= fst e1));
+  |(_, (Dequeue, r)) -> if s = S.empty then None 
+                          else (assume (exists (e:(nat * nat)). S.mem e s /\ (forall e1. S.mem e1 s ==> fst e <= fst e1));
                                 assert (Some? (find_min s));
                                 Some (extract_s (find_min s)))
 
@@ -114,7 +114,430 @@ let resolve_conflict (x:op_t) (y:op_t{fst x <> fst y}) : resolve_conflict_res =
   |(_,(Dequeue,None)), (_,(Dequeue,None)) -> Noop_both
   |(_,(Enqueue _,_)), (_,(Dequeue,Some _)) -> Second_then_first
   |(_,(Dequeue,Some _)), (_,(Enqueue _,_)) -> First_then_second 
-  |(_,(Dequeue,Some _)), (_,(Dequeue,Some _)) -> if x = y then First 
+  |(_,(Dequeue,Some _)), (_,(Dequeue,Some _)) -> if fst (extract x) = fst (extract y) then First 
                                                  else if fst (extract x) < fst (extract y) then First_then_second
                                                       else Second_then_first
  
+let concrete_merge (lca s1 s2:concrete_st) 
+  : Pure concrete_st
+         (requires (exists l1 l2. apply_log lca l1 == s1 /\ apply_log lca l2 == s2))
+         (ensures (fun _ -> True)) =
+  let i' = S.intersect s1 s2 in
+  let i = S.intersect lca i' in
+  let da = S.remove_if s1 (fun e -> S.mem e lca) in
+  let db = S.remove_if s2 (fun e -> S.mem e lca) in
+  S.union i (S.union da db)
+  
+let linearizable_s1_0''_base_base (lca s1 s2':st) (last2:op_t)
+  : Lemma (requires consistent_branches lca s1 s2' /\
+                    is_prefix (ops_of lca) (snoc (ops_of s2') last2) /\
+                    ops_of s1 = ops_of lca /\ ops_of s2' = ops_of lca /\
+                    length (ops_of lca) = 0)
+        
+          (ensures eq (do (v_of s2') last2) (concrete_merge (v_of lca) (v_of s1) (do (v_of s2') last2))) = ()
+
+let linearizable_s1_0''_base_ind (lca s1 s2':st) (last2:op_t)
+  : Lemma (requires consistent_branches lca s1 s2' /\
+                    is_prefix (ops_of lca) (snoc (ops_of s2') last2) /\
+                    ops_of s1 = ops_of lca /\ ops_of s2' = ops_of lca /\
+                    length (ops_of lca) > 0 /\
+                    (forall id. mem_id id (ops_of lca) ==> lt id (fst last2)) /\
+
+                    (let l' = inverse_st lca in
+                    let s1' = inverse_st s1 in
+                    let s2'' = inverse_st s2' in
+                    consistent_branches l' s1' s2'' /\
+                    is_prefix (ops_of l') (snoc (ops_of s2'') last2) /\
+                    ops_of s1' = ops_of l' /\ ops_of s2'' = ops_of l' /\
+                    eq (do (v_of s2'') last2) (concrete_merge (v_of l') (v_of s1') (do (v_of s2'') last2))))
+
+          (ensures eq (do (v_of s2') last2) (concrete_merge (v_of lca) (v_of s1) (do (v_of s2') last2))) = ()
+
+let linearizable_s1_0''_ind (lca s1 s2':st) (last2:op_t)
+  : Lemma (requires consistent_branches_s2_gt0 lca s1 s2' /\
+                    is_prefix (ops_of lca) (snoc (ops_of s2') last2) /\
+                    ops_of s1 = ops_of lca /\
+                    (forall id. mem_id id (ops_of lca) ==> lt id (fst last2)) /\
+
+                    (let inv2 = inverse_st s2' in
+                    consistent_branches lca s1 inv2 /\
+                    is_prefix (ops_of lca) (snoc (ops_of inv2) last2) /\
+                    (exists l2. do (v_of inv2) last2 == apply_log (v_of lca) l2) /\
+                    (exists l2. do (v_of s2') last2 == apply_log (v_of lca) l2) /\                    
+                    eq (do (v_of inv2) last2) (concrete_merge (v_of lca) (v_of s1) (do (v_of inv2) last2))))
+        
+          (ensures eq (do (v_of s2') last2) (concrete_merge (v_of lca) (v_of s1) (do (v_of s2') last2))) = ()
+
+let linearizable_s1_0_s2_0_base (lca s1 s2:st)
+  : Lemma (requires (exists l1. v_of s1 == apply_log (v_of lca) l1) /\
+                    (exists l2. v_of s2 == apply_log (v_of lca) l2) /\
+                    ops_of s1 == ops_of lca /\ ops_of s2 == ops_of lca)
+        
+          (ensures eq (v_of lca) (concrete_merge (v_of lca) (v_of s1) (v_of s2))) = ()
+
+let linearizable_s2_0''_base_base (lca s1' s2:st) (last1:op_t)
+  : Lemma (requires consistent_branches lca s1' s2 /\
+                    is_prefix (ops_of lca) (snoc (ops_of s1') last1) /\
+                    ops_of s1' = ops_of lca /\ ops_of s2 = ops_of lca /\
+                    length (ops_of lca) = 0 /\
+                    (forall id. mem_id id (ops_of lca) ==> lt id (fst last1)))
+         
+          (ensures eq (do (v_of s1') last1) (concrete_merge (v_of lca) (do (v_of s1') last1) (v_of s2))) = ()
+
+let linearizable_s2_0''_base_ind (lca s1' s2:st) (last1:op_t)
+  : Lemma (requires consistent_branches lca s1' s2 /\
+                    is_prefix (ops_of lca) (snoc (ops_of s1') last1) /\
+                    ops_of s1' = ops_of lca /\ ops_of s2 = ops_of lca /\
+                    length (ops_of lca) > 0 /\
+                    (forall id. mem_id id (ops_of lca) ==> lt id (fst last1)) /\
+
+                    (let l' = inverse_st lca in
+                    let s1'' = inverse_st s1' in
+                    let s2' = inverse_st s2 in
+                    consistent_branches l' s1'' s2' /\
+                    is_prefix (ops_of l') (snoc (ops_of s1'') last1) /\
+                    ops_of s1'' = ops_of l' /\ ops_of s2' = ops_of l' /\
+                    eq (do (v_of s1'') last1) (concrete_merge (v_of l') (do (v_of s1'') last1) (v_of s2'))))
+
+          (ensures eq (do (v_of s1') last1) (concrete_merge (v_of lca) (do (v_of s1') last1) (v_of s2))) = ()
+
+let linearizable_s2_0''_ind (lca s1' s2:st) (last1:op_t)
+  : Lemma (requires consistent_branches_s1_gt0 lca s1' s2 /\
+                    is_prefix (ops_of lca) (snoc (ops_of s1') last1) /\
+                    ops_of s2 = ops_of lca /\
+                    (forall id. mem_id id (ops_of lca) ==> lt id (fst last1)) /\
+
+                    (let inv1 = inverse_st s1' in
+                    consistent_branches lca inv1 s2 /\
+                    is_prefix (ops_of lca) (snoc (ops_of inv1) last1) /\
+                    (exists l1. (do (v_of inv1) last1 == apply_log (v_of lca) l1)) /\
+                    (exists l1. (do (v_of s1') last1 == apply_log (v_of lca) l1)) /\
+                    eq (do (v_of inv1) last1) (concrete_merge (v_of lca) (do (v_of inv1) last1) (v_of s2))))
+         
+          (ensures eq (do (v_of s1') last1) (concrete_merge (v_of lca) (do (v_of s1') last1) (v_of s2))) = ()
+
+let linearizable_gt0_base_ee_fts (lca s1 s2:st) (last1 last2:op_t)
+  : Lemma (requires consistent_branches lca s1 s2 /\
+                    ops_of s1 = ops_of lca /\ ops_of s2 = ops_of lca /\
+                    fst last1 <> fst last2 /\ 
+                    (exists l2. (do (v_of s2) last2 == apply_log (v_of lca) l2)) /\
+                    (exists l1. (do (v_of s1) last1 == apply_log (v_of lca) l1)) /\
+                    First_then_second? (resolve_conflict last1 last2) /\
+                    Enqueue? (fst (snd last1)) /\ Enqueue? (fst (snd last2)) /\ fst last1 > fst last2)
+         
+          (ensures eq (do (concrete_merge (v_of lca) (v_of s1) (do (v_of s2) last2)) last1)
+                      (concrete_merge (v_of lca) (do (v_of s1) last1) (do (v_of s2) last2))) = ()
+
+#push-options "--z3rlimit 50"
+let linearizable_gt0_base_de_fts (lca s1 s2:st) (last1 last2:op_t)
+  : Lemma (requires consistent_branches lca s1 s2 /\
+                    ops_of s1 = ops_of lca /\ ops_of s2 = ops_of lca /\
+                    fst last1 <> fst last2 /\ 
+                    (exists l2. (do (v_of s2) last2 == apply_log (v_of lca) l2)) /\
+                    (exists l1. (do (v_of s1) last1 == apply_log (v_of lca) l1)) /\
+                    First_then_second? (resolve_conflict last1 last2) /\
+                    Dequeue? (fst (snd last1)) /\ Some? (ret_of last1) /\ Enqueue? (fst (snd last2)))
+         
+          (ensures (eq (do (concrete_merge (v_of lca) (v_of s1) (do (v_of s2) last2)) last1)
+                       (concrete_merge (v_of lca) (do (v_of s1) last1) (do (v_of s2) last2)))) = 
+  assume (unique_st (v_of lca) /\ unique_st (v_of s1) /\ unique_st (v_of s2)); //todo
+  assume (ret_of last1 = return (v_of s1) last1); //to include in pre-cond    
+  assume (ret_of last2 = return (v_of s2) last2); //to include in pre-cond  
+  assume (forall id. mem_id_s id (v_of s2) ==> fst last2 > id);
+  ()
+
+let linearizable_gt0_base_dd_fts (lca s1 s2:st) (last1 last2:op_t)
+  : Lemma (requires consistent_branches lca s1 s2 /\
+                    ops_of s1 = ops_of lca /\ ops_of s2 = ops_of lca /\
+                    fst last1 <> fst last2 /\ 
+                    (exists l2. (do (v_of s2) last2 == apply_log (v_of lca) l2)) /\
+                    (exists l1. (do (v_of s1) last1 == apply_log (v_of lca) l1)) /\
+                    First_then_second? (resolve_conflict last1 last2) /\
+                    Dequeue? (fst (snd last1)) /\ Some? (ret_of last1) /\ 
+                    Dequeue? (fst (snd last2)) /\ Some? (ret_of last2) /\
+                    fst (extract last1) < fst (extract last2))
+         
+          (ensures (eq (do (concrete_merge (v_of lca) (v_of s1) (do (v_of s2) last2)) last1)
+                       (concrete_merge (v_of lca) (do (v_of s1) last1) (do (v_of s2) last2)))) = 
+  assume (unique_st (v_of lca) /\ unique_st (v_of s1) /\ unique_st (v_of s2)); //todo
+  assume (ret_of last1 = return (v_of s1) last1); //to include in pre-cond    
+  assume (ret_of last2 = return (v_of s2) last2); //to include in pre-cond  
+  ()
+
+let linearizable_gt0_base_fts (lca s1 s2:st) (last1 last2:op_t)
+  : Lemma (requires consistent_branches lca s1 s2 /\
+                    ops_of s1 = ops_of lca /\ ops_of s2 = ops_of lca /\
+                    fst last1 <> fst last2 /\ 
+                    (exists l2. (do (v_of s2) last2 == apply_log (v_of lca) l2)) /\
+                    (exists l1. (do (v_of s1) last1 == apply_log (v_of lca) l1)) /\
+                    First_then_second? (resolve_conflict last1 last2))
+         
+          (ensures (eq (do (concrete_merge (v_of lca) (v_of s1) (do (v_of s2) last2)) last1)
+                       (concrete_merge (v_of lca) (do (v_of s1) last1) (do (v_of s2) last2)))) =
+  if Enqueue? (fst (snd last1)) && Enqueue? (fst (snd last2)) && fst last1 > fst last2 then
+    linearizable_gt0_base_ee_fts lca s1 s2 last1 last2
+  else if Dequeue? (fst (snd last1)) && Some? (ret_of last1) && Enqueue? (fst (snd last2)) then
+    linearizable_gt0_base_de_fts lca s1 s2 last1 last2
+  else linearizable_gt0_base_dd_fts lca s1 s2 last1 last2
+
+let linearizable_gt0_base_ee_stf (lca s1 s2:st) (last1 last2:op_t)
+  : Lemma (requires consistent_branches lca s1 s2 /\
+                    ops_of s1 = ops_of lca /\ ops_of s2 = ops_of lca /\
+                    fst last1 <> fst last2 /\ 
+                    (exists l2. (do (v_of s2) last2 == apply_log (v_of lca) l2)) /\
+                    (exists l1. (do (v_of s1) last1 == apply_log (v_of lca) l1)) /\
+                    Second_then_first? (resolve_conflict last1 last2) /\
+                    Enqueue? (fst (snd last1)) /\ Enqueue? (fst (snd last2)) /\ fst last1 < fst last2)
+         
+          (ensures eq (do (concrete_merge (v_of lca) (do (v_of s1) last1) (v_of s2)) last2)
+                      (concrete_merge (v_of lca) (do (v_of s1) last1) (do (v_of s2) last2))) = ()
+
+let linearizable_gt0_base_de_stf (lca s1 s2:st) (last1 last2:op_t)
+  : Lemma (requires consistent_branches lca s1 s2 /\
+                    ops_of s1 = ops_of lca /\ ops_of s2 = ops_of lca /\
+                    fst last1 <> fst last2 /\ 
+                    (exists l2. (do (v_of s2) last2 == apply_log (v_of lca) l2)) /\
+                    (exists l1. (do (v_of s1) last1 == apply_log (v_of lca) l1)) /\
+                    Second_then_first? (resolve_conflict last1 last2) /\
+                    Dequeue? (fst (snd last2)) /\ Some? (ret_of last2) /\ Enqueue? (fst (snd last1)))
+         
+          (ensures eq (do (concrete_merge (v_of lca) (do (v_of s1) last1) (v_of s2)) last2)
+                      (concrete_merge (v_of lca) (do (v_of s1) last1) (do (v_of s2) last2))) = 
+  assume (unique_st (v_of lca) /\ unique_st (v_of s1) /\ unique_st (v_of s2)); //todo
+  assume (ret_of last1 = return (v_of s1) last1); //to include in pre-cond    
+  assume (ret_of last2 = return (v_of s2) last2); //to include in pre-cond  
+  assume (forall id. mem_id_s id (v_of s1) ==> fst last1 > id);
+  ()
+
+let linearizable_gt0_base_dd_stf (lca s1 s2:st) (last1 last2:op_t)
+  : Lemma (requires consistent_branches lca s1 s2 /\
+                    ops_of s1 = ops_of lca /\ ops_of s2 = ops_of lca /\
+                    fst last1 <> fst last2 /\ 
+                    (exists l2. (do (v_of s2) last2 == apply_log (v_of lca) l2)) /\
+                    (exists l1. (do (v_of s1) last1 == apply_log (v_of lca) l1)) /\
+                    Second_then_first? (resolve_conflict last1 last2) /\
+                    Dequeue? (fst (snd last1)) /\ Some? (ret_of last1) /\ 
+                    Dequeue? (fst (snd last2)) /\ Some? (ret_of last2) /\
+                    fst (extract last1) >= fst (extract last2))
+         
+          (ensures eq (do (concrete_merge (v_of lca) (do (v_of s1) last1) (v_of s2)) last2)
+                      (concrete_merge (v_of lca) (do (v_of s1) last1) (do (v_of s2) last2))) = 
+   assume (unique_st (v_of lca) /\ unique_st (v_of s1) /\ unique_st (v_of s2)); //todo
+   assume (ret_of last1 = return (v_of s1) last1); //to include in pre-cond    
+   assume (ret_of last2 = return (v_of s2) last2); //to include in pre-cond  
+   ()
+
+let linearizable_gt0_base_stf (lca s1 s2:st) (last1 last2:op_t)
+  : Lemma (requires consistent_branches lca s1 s2 /\
+                    ops_of s1 = ops_of lca /\ ops_of s2 = ops_of lca /\
+                    fst last1 <> fst last2 /\ 
+                    (exists l2. (do (v_of s2) last2 == apply_log (v_of lca) l2)) /\
+                    (exists l1. (do (v_of s1) last1 == apply_log (v_of lca) l1)) /\
+                    Second_then_first? (resolve_conflict last1 last2))
+         
+          (ensures eq (do (concrete_merge (v_of lca) (do (v_of s1) last1) (v_of s2)) last2)
+                      (concrete_merge (v_of lca) (do (v_of s1) last1) (do (v_of s2) last2))) =
+  if Enqueue? (fst (snd last1)) && Enqueue? (fst (snd last2)) && fst last1 < fst last2 then
+    linearizable_gt0_base_ee_stf lca s1 s2 last1 last2
+  else if Dequeue? (fst (snd last2)) && Some? (ret_of last2) && Enqueue? (fst (snd last1)) then
+    linearizable_gt0_base_de_stf lca s1 s2 last1 last2
+  else linearizable_gt0_base_dd_stf lca s1 s2 last1 last2
+  
+let linearizable_gt0_base (lca s1 s2:st) (last1 last2:op_t)
+  : Lemma (requires consistent_branches lca s1 s2 /\
+                    ops_of s1 = ops_of lca /\ ops_of s2 = ops_of lca /\
+                    fst last1 <> fst last2 /\ 
+                    (exists l2. (do (v_of s2) last2 == apply_log (v_of lca) l2)) /\
+                    (exists l1. (do (v_of s1) last1 == apply_log (v_of lca) l1)))
+         
+          (ensures (First_then_second? (resolve_conflict last1 last2) ==>
+                      (eq (do (concrete_merge (v_of lca) (v_of s1) (do (v_of s2) last2)) last1)
+                         (concrete_merge (v_of lca) (do (v_of s1) last1) (do (v_of s2) last2)))) /\
+
+                   (Second_then_first? (resolve_conflict last1 last2) ==>
+                      (eq (do (concrete_merge (v_of lca) (do (v_of s1) last1) (v_of s2)) last2)
+                         (concrete_merge (v_of lca) (do (v_of s1) last1) (do (v_of s2) last2))))) = admit()
+
+let linearizable_gt0_ind (lca s1 s2:st) (last1 last2:op_t)
+  : Lemma (requires consistent_branches_s2_gt0 lca s1 s2 /\
+                    fst last1 <> fst last2 /\
+                    distinct_ops (snoc (ops_of s1) last1) /\
+                    distinct_ops (snoc (ops_of s2) last2) /\
+                    (exists l1. (do (v_of s1) last1 == apply_log (v_of lca) l1)) /\
+                    (exists l2. (do (v_of s2) last2 == apply_log (v_of lca) l2)) /\
+                    (let s2' = inverse_st s2 in
+                    (exists l2. (do (v_of s2') last2 == apply_log (v_of lca) l2)) /\
+                    (exists l2. (v_of s2' == apply_log (v_of lca) l2)) /\
+                    (exists l1. (v_of s1 == apply_log (v_of lca) l1)) /\
+                    (exists l2. (v_of s2 == apply_log (v_of lca) l2)) /\
+                    consistent_branches lca s1 s2'))
+       
+          (ensures (let s2' = inverse_st s2 in
+                   ((First_then_second? (resolve_conflict last1 last2) /\
+                    eq (do (concrete_merge (v_of lca) (v_of s1) (do (v_of s2') last2)) last1)
+                       (concrete_merge (v_of lca) (do (v_of s1) last1) (do (v_of s2') last2))) ==>
+                    (eq (do (concrete_merge (v_of lca) (v_of s1) (do (v_of s2) last2)) last1)
+                        (concrete_merge (v_of lca) (do (v_of s1) last1) (do (v_of s2) last2)))) /\
+                          
+                   ((ops_of s1 = ops_of lca /\
+                    Second_then_first? (resolve_conflict last1 last2) /\
+                    eq (do (concrete_merge (v_of lca) (do (v_of s1) last1) (v_of s2')) last2)
+                       (concrete_merge (v_of lca) (do (v_of s1) last1) (do (v_of s2') last2))) ==>
+                    (eq (do (concrete_merge (v_of lca) (do (v_of s1) last1) (v_of s2)) last2)
+                        (concrete_merge (v_of lca) (do (v_of s1) last1) (do (v_of s2) last2)))))) = admit()
+
+let linearizable_gt0_ind1 (lca s1 s2:st) (last1 last2:op_t)
+  : Lemma (requires consistent_branches_s1_gt0 lca s1 s2 /\
+                    fst last1 <> fst last2 /\
+                    distinct_ops (snoc (ops_of s1) last1) /\
+                    distinct_ops (snoc (ops_of s2) last2) /\
+                    (exists l1. (do (v_of s1) last1 == apply_log (v_of lca) l1)) /\
+                    (exists l2. (do (v_of s2) last2 == apply_log (v_of lca) l2)) /\
+                    (let s1' = inverse_st s1 in
+                    (exists l1. (do (v_of s1') last1 == apply_log (v_of lca) l1)) /\
+                    (exists l1. (v_of s1' == apply_log (v_of lca) l1)) /\
+                    (exists l1. (v_of s1 == apply_log (v_of lca) l1)) /\
+                    (exists l2. (v_of s2 == apply_log (v_of lca) l2)) /\
+                    consistent_branches lca s1' s2))
+        
+          (ensures (let s1' = inverse_st s1 in
+                   ((ops_of s2 = ops_of lca /\
+                   First_then_second? (resolve_conflict last1 last2) /\
+                   eq (do (concrete_merge (v_of lca) (v_of s1') (do (v_of s2) last2)) last1)
+                      (concrete_merge (v_of lca) (do (v_of s1') last1) (do (v_of s2) last2))) ==>
+                   eq (do (concrete_merge (v_of lca) (v_of s1) (do (v_of s2) last2)) last1)
+                      (concrete_merge (v_of lca) (do (v_of s1) last1) (do (v_of s2) last2))) /\
+
+                   ((Second_then_first? (resolve_conflict last1 last2) /\
+                    eq (do (concrete_merge (v_of lca) (do (v_of s1') last1) (v_of s2)) last2)
+                       (concrete_merge (v_of lca) (do (v_of s1') last1) (do (v_of s2) last2)) ==>
+                    eq (do (concrete_merge (v_of lca) (do (v_of s1) last1) (v_of s2)) last2)
+                       (concrete_merge (v_of lca) (do (v_of s1) last1) (do (v_of s2) last2)))))) = admit()
+
+let linearizable_gt0_s1's2' (lca s1 s2:st)
+  : Lemma (requires consistent_branches_s1s2_gt0 lca s1 s2 /\ 
+                    (let _, last1 = un_snoc (ops_of s1) in
+                     let _, last2 = un_snoc (ops_of s2) in
+                     fst last1 <> fst last2 /\
+                     First? (resolve_conflict last1 last2) /\
+                     (exists l1. (v_of s1 == apply_log (v_of lca) l1)) /\
+                     (exists l2. (v_of s2 == apply_log (v_of lca) l2)) /\
+                     (exists l1. (v_of (inverse_st s1) == apply_log (v_of lca) l1)) /\
+                     (exists l2. (v_of (inverse_st s2) == apply_log (v_of lca) l2)) /\
+                     is_prefix (ops_of lca) (ops_of (inverse_st s2)) /\
+                     is_prefix (ops_of lca) (ops_of (inverse_st s1))))
+          (ensures (let _, last1 = un_snoc (ops_of s1) in
+                    eq (do (concrete_merge (v_of lca) (v_of (inverse_st s1)) (v_of (inverse_st s2))) last1)
+                       (concrete_merge (v_of lca) (v_of s1) (v_of s2)))) = 
+   assume (unique_st (v_of lca) /\ unique_st (v_of s1) /\ unique_st (v_of s2)); //todo
+   lem_apply_log init_st (ops_of s1);
+   lem_apply_log init_st (ops_of s2);
+   admit()
+
+let linearizable_gt0_s1'_noop (lca s1 s2:st)
+  : Lemma (requires consistent_branches_s1s2_gt0 lca s1 s2 /\ 
+                    (let _, last1 = un_snoc (ops_of s1) in
+                     let _, last2 = un_snoc (ops_of s2) in
+                     fst last1 <> fst last2 /\
+                     Noop_first? (resolve_conflict last1 last2) /\
+                     (exists l1. (v_of s1 == apply_log (v_of lca) l1)) /\
+                     (exists l2. (v_of s2 == apply_log (v_of lca) l2)) /\
+                     (exists l1. (v_of (inverse_st s1) == apply_log (v_of lca) l1)) /\
+                     is_prefix (ops_of lca) (ops_of (inverse_st s1))))
+          (ensures eq (concrete_merge (v_of lca) (v_of (inverse_st s1)) (v_of s2))
+                      (concrete_merge (v_of lca) (v_of s1) (v_of s2))) = 
+  assume (unique_st (v_of lca) /\ unique_st (v_of s1) /\ unique_st (v_of s2)); //todo
+  lem_apply_log init_st (ops_of s1)
+
+let linearizable_gt0_s2'_noop (lca s1 s2:st)
+  : Lemma (requires consistent_branches_s1s2_gt0 lca s1 s2 /\ 
+                    (let _, last1 = un_snoc (ops_of s1) in
+                     let _, last2 = un_snoc (ops_of s2) in
+                     fst last1 <> fst last2 /\
+                     Noop_second? (resolve_conflict last1 last2) /\
+                     (exists l1. (v_of s1 == apply_log (v_of lca) l1)) /\
+                     (exists l2. (v_of s2 == apply_log (v_of lca) l2)) /\
+                     (exists l2. (v_of (inverse_st s2) == apply_log (v_of lca) l2)) /\
+                     is_prefix (ops_of lca) (ops_of (inverse_st s2))))
+          (ensures eq (concrete_merge (v_of lca) (v_of s1) (v_of (inverse_st s2)))
+                      (concrete_merge (v_of lca) (v_of s1) (v_of s2))) = 
+  assume (unique_st (v_of lca) /\ unique_st (v_of s1) /\ unique_st (v_of s2)); //todo
+  lem_apply_log init_st (ops_of s2)
+  
+let linearizable_gt0_s1's2'_noop_both (lca s1 s2:st)
+  : Lemma (requires consistent_branches_s1s2_gt0 lca s1 s2 /\ 
+                    (let _, last1 = un_snoc (ops_of s1) in
+                     let _, last2 = un_snoc (ops_of s2) in
+                     fst last1 <> fst last2 /\
+                     Noop_both? (resolve_conflict last1 last2) /\
+                     (exists l1. (v_of s1 == apply_log (v_of lca) l1)) /\
+                     (exists l2. (v_of s2 == apply_log (v_of lca) l2)) /\
+                     (exists l1. (v_of (inverse_st s1) == apply_log (v_of lca) l1)) /\
+                     (exists l2. (v_of (inverse_st s2) == apply_log (v_of lca) l2)) /\
+                     is_prefix (ops_of lca) (ops_of (inverse_st s2)) /\
+                     is_prefix (ops_of lca) (ops_of (inverse_st s1))))
+          (ensures eq (concrete_merge (v_of lca) (v_of (inverse_st s1)) (v_of (inverse_st s2)))
+                      (concrete_merge (v_of lca) (v_of s1) (v_of s2))) = ()
+
+
+////////////////////////////////////////////////////////////////
+//// Sequential implementation //////
+
+// the concrete state 
+type concrete_st_s = S.set nat
+
+// init state 
+let init_st_s = S.empty
+
+let find_min_seq (s:concrete_st_s)
+    : (m:option nat
+           {(Some? m <==> (exists (e:(nat)). S.mem e s /\ (forall e1. S.mem e1 s ==> e <= e1))) /\
+            (Some? m ==> (exists (e:(nat)). S.mem e s /\ (forall e1. S.mem e1 s ==> e <= e1) /\ e = extract_s m)) /\
+        (s = S.empty ==> (m = None \/ (~ (exists (e:(nat)). S.mem e s /\ (forall e1. S.mem e1 s ==> e <= e1))))) 
+        (*s <> empty ==> Some? m*)}) =
+  S.find_if s (fun e -> (S.forall_s s (fun e1 -> e <= e1)))
+  
+let remove_min_seq (s:concrete_st_s) 
+  : (r:concrete_st_s{(s = S.empty ==> r = s) /\
+                   (s <> S.empty /\ Some? (find_min_seq s) ==> (forall e. S.mem e r <==> (S.mem e s /\ e <> extract_s (find_min_seq s)))) /\
+                   (s <> S.empty /\ None? (find_min_seq s) ==> (forall e. S.mem e r <==> S.mem e s))}) =
+  if s = S.empty then s 
+  else (let m = find_min_seq s in
+        if Some? m then S.remove_if s (fun e -> e = extract_s (find_min_seq s))
+        else s)
+        
+// apply an operation to a state 
+let do_s (s:concrete_st_s) (op:op_t) : concrete_st_s = 
+  match op with
+  |(id, (Enqueue x, _)) -> S.add x s
+  |(_, (Dequeue, _)) -> if s = S.empty then s else remove_min_seq s
+  
+//equivalence relation between the concrete states of sequential type and MRDT
+let eq_sm (st_s:concrete_st_s) (st:concrete_st) : Tot prop =
+  (forall e. S.mem e st ==> S.mem (snd e) st_s) /\
+  (forall e. S.mem e st_s ==> (exists id. S.mem (id, e) st))
+
+//initial states are equivalent
+let initial_eq _
+  : Lemma (ensures eq_sm init_st_s init_st) = ()
+
+let min_same (st_s:concrete_st_s) (st:concrete_st) 
+  : Lemma (requires eq_sm st_s st)
+          (ensures (None? (find_min_seq st_s) <==> None? (find_min st)) /\
+                   (Some? (find_min_seq st_s) <==> Some? (find_min st)) /\
+                   (Some? (find_min_seq st_s) ==> extract_s (find_min_seq st_s) = snd (extract_s (find_min st)))) = admit()
+
+let remove_same (st_s:concrete_st_s) (st:concrete_st) 
+  : Lemma (requires eq_sm st_s st)
+          (ensures (eq_sm (remove_min_seq st_s) (remove_min st))) =
+  admit();min_same st_s st
+ 
+//equivalence between states of sequential type and MRDT at every operation
+let do_eq (st_s:concrete_st_s) (st:concrete_st) (op:op_t)
+  : Lemma (requires eq_sm st_s st)
+          (ensures eq_sm (do_s st_s op) (do st op)) =
+  min_same st_s st;
+  remove_same st_s st;
+  if Enqueue? (fst (snd op)) then () else ()
+  
+////////////////////////////////////////////////////////////////
